src/tree/TreeData.dfy
@@ -1,0 +1,93 @@
+datatype tree<A> = Empty | Node(left: tree<A>, data: A, right: tree<A>)
+
+function method Leaf<A>(d: A): tree<A>
+{
+  Node(Empty, d, Empty)
+}
+
+function method elems<A>(t: tree<A>): set<A>
+  ensures t.Empty? ==> elems(t) == {}
+  ensures !t.Empty? ==> elems(t) == elems(t.left) + {t.data} + elems(t.right)
+{
+  match t {
+    case Empty => {}
+    case Node(l, x, r) => elems(l) + {x} + elems(r)
+  }
+}
+
+function method elemsDownTo<A>(t: tree<A>, d: nat): set<A>
+{
+  if d == 0 || t.Empty? then
+    {}
+  else
+    elemsDownTo(t.left, d-1) + {t.data} + elemsDownTo(t.right, d-1)
+}
+
+function method melems<A>(t: tree<A>): multiset<A>
+{
+  match t {
+    case Empty => multiset{}
+    case Node(l, x, r) => melems(l) + multiset{x} + melems(r)
+  }
+}
+
+function method fmap<A, B>(t: tree<A>, f: A -> B): tree<B>
+{
+  match t {
+    case Empty() => Empty()
+    case Node(l, x, r) => Node(fmap(l, f), f(x), fmap(r, f))
+  }
+}
+
+function method preorder<A>(t: tree<A>): seq<A>
+{
+  match t {
+    case Empty => []
+    case Node(l, x, r) => [x] + preorder(l) + preorder(r)
+  }
+}
+
+function method inorder<A>(t: tree<A>): seq<A>
+{
+  match t {
+    case Empty => []
+    case Node(l, x, r) => inorder(l) + [x] + inorder(r)
+  }
+}
+
+function method revinorder<A>(t: tree<A>): seq<A>
+{
+  match t {
+    case Empty => []
+    case Node(l, x, r) => revinorder(r) + [x] + revinorder(l)
+  }
+}
+
+function method postorder<A>(t: tree<A>): seq<A>
+{
+  match t {
+    case Empty => []
+    case Node(l, x, r) => postorder(l) + postorder(r) + [x]
+  }
+}
+
+function method size<A>(t: tree<A>): nat
+{
+  |preorder(t)|
+}
+
+function method max(x: int, y: int): int
+{
+  if x < y then
+    y
+  else
+    x
+}
+
+function method depth<A>(t: tree<A>): nat
+{
+  match t {
+    case Empty => 0
+    case Node(l, x, r) => max(depth(l), depth(r)) + 1
+  }
+}
